src/program_proof/simplepb/primary_protocol.v
@@ -1,0 +1,166 @@
+From Perennial.program_proof Require Import grove_prelude.
+From iris.base_logic Require Export lib.ghost_var mono_nat.
+From iris.algebra Require Import dfrac_agree mono_list csum.
+From Perennial.program_proof.simplepb Require Import pb_protocol.
+
+Section primary_protocol.
+
+Context `{EntryType}.
+
+Record primary_system_names :=
+{
+  prim_init_proposal_gn : gname ;
+}.
+
+Record primary_server_names :=
+{
+  prim_escrow_gn : gname ; (* escrow for getting ownership of proposal *)
+}.
+
+Class primary_ghostG Σ := {
+    primary_ghost_map_logG :> fmlist_mapG Σ u64 EntryType;
+    primary_escrowG :> inG Σ (gmapR u64 (dfrac_agreeR unitO))
+}.
+
+Context `{!primary_ghostG Σ}.
+Context `{!gooseGlobalGS Σ}.
+
+Implicit Type γsrv : primary_server_names.
+Implicit Type γsys : primary_system_names.
+Implicit Type σ : list EntryType.
+Implicit Type epoch : u64.
+
+Notation "lhs ⪯ rhs" := (prefix lhs rhs)
+(at level 20, format "lhs  ⪯  rhs") : stdpp_scope.
+
+(* FIXME: ideally, this init proposal stuff and the escrow tokens should be a
+   separate higher-level protocol *)
+Definition own_init_proposal_unused γsys epoch : iProp Σ :=
+  epoch ⤳l[γsys.(prim_init_proposal_gn)] [].
+Definition is_init_proposal γsys epoch σ : iProp Σ :=
+  epoch ⤳l[γsys.(prim_init_proposal_gn)]□ σ.
+Definition is_init_proposal_ub γsys epoch σ : iProp Σ :=
+  ∃ σexact,
+  ⌜σexact ⪯ σ⌝ ∗
+  is_init_proposal γsys epoch σexact.
+
+Definition own_tok γsrv epoch : iProp Σ :=
+  own γsrv.(prim_escrow_gn) {[ epoch := to_dfrac_agree (DfracOwn 1) ()]}.
+
+Definition is_tok γsrv epoch : iProp Σ :=
+  own γsrv.(prim_escrow_gn) {[ epoch := to_dfrac_agree (DfracDiscarded) ()]}.
+
+Definition is_proposal_facts_prim γ epoch σ: iProp Σ :=
+  is_init_proposal_ub γ epoch σ
+.
+
+Definition own_escrow_toks γsrv epoch : iProp Σ :=
+  [∗ set] epoch' ∈ (fin_to_set u64), ⌜int.nat epoch' ≤ int.nat epoch⌝ ∨ own_tok γsrv epoch'
+.
+
+Definition own_primary_ghost γsys γsrv (canBecomePrimary:bool) epoch : iProp Σ :=
+  "Htoks" ∷ own_escrow_toks γsrv epoch ∗
+  "Htok" ∷ (if canBecomePrimary then own_tok γsrv epoch else True)
+.
+
+Lemma ghost_primary_accept_new_epoch γsys γsrv epoch canBecomePrimary epoch' :
+  int.nat epoch < int.nat epoch' →
+  own_primary_ghost γsys γsrv canBecomePrimary epoch
+  ==∗
+  own_primary_ghost γsys γsrv true epoch'.
+Proof.
+  (*
+  intros Hineq.
+  iIntros "#Hprop_facts #Hprop_lb".
+  iNamed 1.
+  iClear "Hprop".
+  iDestruct (big_sepS_elem_of_acc_impl epoch' with "Htoks") as "[Htok Htoks]".
+  { set_solver. }
+  iDestruct "Htok" as "[%Hbad|Htok]".
+  { exfalso. word. }
+  iFrame "Htok Hprop_facts Hprop_lb".
+  iApply "Htoks".
+  {
+    iModIntro.
+    iIntros (???) "[%Hineq2|$]".
+    iLeft.
+    iPureIntro.
+    word.
+  }
+  {
+    iModIntro. iLeft.
+    done.
+  } *)
+Admitted.
+
+Lemma own_tok_is_tok_false γ epoch :
+  own_tok γ epoch -∗
+  is_tok γ epoch -∗
+  False.
+Proof.
+  iIntros "Htok His".
+  iDestruct (own_valid_2 with "His Htok") as %Hbad.
+  rewrite singleton_op singleton_valid dfrac_agree_op_valid in Hbad.
+  naive_solver.
+Qed.
+
+Lemma primary_ghost_init_primary γsys γsrv σ epoch_new :
+  own_init_proposal_unused γsys epoch_new
+  ==∗
+  is_init_proposal γsys epoch_new σ
+.
+Proof.
+  iIntros "Hinit".
+  iMod (fmlist_ptsto_update σ with "Hinit") as "Hinit".
+  { apply prefix_nil. }
+  iMod (fmlist_ptsto_persist with "Hinit") as "#Hinit".
+  done.
+Qed.
+
+Definition become_primary_escrow γsys γsrv epoch σ R : iProp Σ :=
+  is_init_proposal γsys epoch σ ∗
+  inv pbN (R ∨ is_tok γsrv epoch)
+.
+
+Lemma ghost_become_primary γsys γsrv epoch σprop σ R :
+  £ 1 -∗
+  become_primary_escrow γsys γsrv epoch σprop R -∗
+  is_proposal_facts_prim γsys epoch σ -∗
+  own_primary_ghost γsys γsrv true epoch ={↑pbN}=∗
+  ⌜σprop ⪯ σ⌝ ∗
+  own_primary_ghost γsys γsrv false epoch ∗
+  R
+.
+Proof.
+  iIntros "Hlc #Hescrow #Hinit_ub".
+  iNamed 1.
+  iDestruct "Hescrow" as "[#Hinit Hescrow]".
+  iInv "Hescrow" as "Hown" "Hclose".
+  iMod (lc_fupd_elim_later with "Hlc Hown" ) as "Hown".
+  iDestruct "Hown" as "[HR|#His_primary]"; last first.
+  { (* contradiction, since we still have the token *)
+    iDestruct (own_valid_2 with "Htok His_primary") as %Hbad.
+    exfalso.
+    rewrite singleton_op singleton_valid dfrac_agree_op_valid in Hbad.
+    destruct Hbad as [Hbad _].
+    done.
+  }
+
+  iFrame "HR".
+  iMod (own_update with "Htok") as "His_primary".
+  {
+    apply singleton_update.
+    apply dfrac_agree_persist.
+  }
+  iDestruct "His_primary" as "#His_primary".
+  iMod ("Hclose" with "[$His_primary]").
+  iModIntro.
+
+  iDestruct "Hinit_ub" as (?) "[%Hineq Hinit2]".
+  iDestruct (fmlist_ptsto_agree with "Hinit Hinit2") as %Heq.
+  subst.
+  iSplitR; first done.
+  iFrame.
+Qed.
+
+End primary_protocol.
